Latest changes

apa.v
@@ -3,6 +3,9 @@ Require Import Coq.Lists.List.
 Require Export ListSet.
 Require Export Arith.
 Require Import Coq.Arith.Peano_dec.
+Require Import Coq.Logic.Classical_Prop.
+Require Import Coq.Logic.Classical_Pred_Type.
+Require Import task.
 Require Import job.
 Require Import schedule.
 Require Import priority.
@@ -12,11 +15,11 @@ Require Import identmp.
 (* Set of all possible affinities (mappings from jobs to processors) *)
 Definition affinity := job -> set nat.
 
-Axiom affinity_non_empty : forall (alpha: affinity) (j: job), ~alpha j = empty_set nat.
+Definition affinity_non_empty := forall (alpha: affinity) (j: job), ~alpha j = empty_set nat.
 
 (* Whether a schedule is produced by an APA identical multiprocessor *)
-Record apa_ident_mp (num_cpus: nat) (sched: schedule)
-                    (alpha: affinity) (hp: higher_priority) : Prop :=
+Record apa_ident_mp (num_cpus: nat) (sched: schedule) (hp: higher_priority)
+                    (cpumap: processor_list) (alpha: affinity) : Prop :=
   {
     (* An identical multiprocessor has a fixed number of cpus *)
     apa_ident_mp_cpus_nonzero: num_cpus > 0;
@@ -24,10 +27,11 @@ Record apa_ident_mp (num_cpus: nat) (sched: schedule)
 
     (* Job is scheduled iff it is mapped to a processor*)
     apa_ident_mp_mapping: forall (j: job) (t: time),
-                              List.In (Some j) (cpumap sched t) <-> sched j t = 1;
+                              List.In (Some j) (cpumap sched t)
+                                  <-> scheduled sched j t;
 
-    (* A scheduled job only receives 1 unit of service *)
-    apa_ident_mp_sched_unit: forall (j: job) (t: time), sched j t <= 1;
+    (* A job receives at most 1 unit of service *)
+    apa_ident_mp_sched_unit: forall (j: job) (t: time), service_at sched j t <= 1;
 
     (* If a job is scheduled, then its affinity should allow it. *)
     apa_ident_mp_restricted_affinities:
@@ -39,7 +43,7 @@ Record apa_ident_mp (num_cpus: nat) (sched: schedule)
         forall (jlow: job) (t: time),
             backlogged sched jlow t <->
                 (forall (cpu: nat),
-                cpu < num_cpus /\
+                cpu < num_cpus ->
                 List.In cpu (alpha jlow) ->
                     (exists (jhigh: job),
                         hp jhigh jlow sched t
@@ -49,35 +53,95 @@ Record apa_ident_mp (num_cpus: nat) (sched: schedule)
 (* Proof that an APA multiprocessor with global affinities is the same as
    an identical multiprocessor with equal number of cpus *)
 Lemma exists_apa_platform_that_is_global :
-    forall (num_cpus: nat) (sched: schedule) (hp: higher_priority),
-        ident_mp num_cpus sched hp ->
-        exists (sched': schedule) (alpha: affinity),
-            apa_ident_mp num_cpus sched alpha hp
-            /\ (forall (j: job) (t: time), service sched j t = service sched' j t).
-Proof. intros. inversion H. exists sched. exists (fun (j : job) => (seq 0 num_cpus)).
-       split. split.
-       apply ident_mp_cpus_nonzero.
-       apply ident_mp_num_cpus.
-       apply ident_mp_mapping.
-       apply ident_mp_sched_unit.
-       intros. apply nat_seq_nth_In.
-       rewrite <- (ident_mp_num_cpus t). apply element_in_list_no_overflow with (x := j).
-       apply H0.
-       intros. assert (H1 := ident_mp_invariant jlow t).
-       inversion H1. split.
-       intros. assert (H5 := H0 H3 cpu). inversion H4.
-       apply H5 in H6. trivial.
-       intros. apply H2. intros.
-       assert (H5 := H3 cpu). assert (H6 := nat_seq_nth_In num_cpus cpu H4).
-       assert (H7 := H5 (conj H4 H6)). trivial. trivial.
-Qed.
+    forall (num_cpus: nat) (sched: schedule) (hp: higher_priority) (cpumap: processor_list),
+        ident_mp num_cpus sched hp cpumap ->
+        schedule_independent hp ->
+        exists (alpha: affinity),
+            forall (sched': schedule) (cpumap': processor_list),
+                apa_ident_mp num_cpus sched' hp cpumap' alpha ->
+                arr_seq sched = arr_seq sched' ->
+                    (forall (j: job) (t: time), service sched j t = service sched' j t).
+Proof. intros num_cpus sched hp cpumap sched_is_identmp sched_ind.
+       inversion_clear sched_is_identmp as [num_cpus_positive _ _ _ invariant_sched].
+       exists (fun (j : job) => (seq 0 num_cpus)).
+       intros sched' cpumap' sched'_is_apa same_arr j t.
+       inversion_clear sched'_is_apa as [num_cpus_sched' _ _ _ _ invariant_sched'].
+       specialize (invariant_sched j t).
+       specialize (invariant_sched' j t).
+
+       induction t.
+       intros.
+       simpl.
+       destruct (excluded_middle (backlogged sched j 0)) as [j_backlogged_sched | j_not_backlogged_sched].
+       destruct (excluded_middle (backlogged sched' j 0)) as [j_backlogged_sched' | j_not_backlogged_sched'].
+
+       - rewrite 2 backlogged_no_service; trivial.
+       - rewrite 2 backlogged_no_service; trivial.
+         apply invariant_sched'. intros cpu cpu_less in_cpu.
+         inversion_clear invariant_sched as [invariant_sched_suf _].
+         specialize (invariant_sched_suf j_backlogged_sched).
+
+         assert (bla : forall cpu0 : nat, 
+                      cpu0 < num_cpus ->
+                      exists jhigh : job,
+                        hp jhigh j sched' 0 /\
+                        exists cpu', cpu' < num_cpus /\ nth cpu' (cpumap sched' 0) None = Some jhigh).
+         admit.
+         apply (bla cpu cpu_less).
+
+         assert (bla := invariant_sched_j_suf cpu cpu_less).
+         inversion bla as [jhigh [H1 H2]].
+         assert (H00 : ~backlogged sched' jhigh 0).
+         rewrite invariant_sched'.
+         unfold not. intros.
+
+         inversion_clear invariant_sched' as [_ invariant_sched'_nec].
+         apply invariant_sched'_nec.
+
+         intros.
+         specialize (invariant_sched_suf cpu H).
+
+
+
+
+         induction cpu.
+             intros.
+             specialize (invariant_sched_suf 0 H).
+             inversion invariant_sched_suf as [jhigh [H1 H2]].
+             destruct (excluded_middle (backlogged sched' jhigh 0)).
+         apply contrapositive in invariant_sched'_nec; trivial.
+         apply invariant_sched'_nec.
+         intros cpu cpu_less in_cpu.
+         
+
+inversion invariant_sched' as [_ invariant_sched'_nec].
+         
+         
+         apply contrapositive in invariant_sched'_nec; trivial.
+         
+         apply not_all_ex_not in invariant_sched'_nec.
+         inversion invariant_sched'_nec as [cpu invariant_neg].
+         apply imply_to_and in invariant_neg.
+         inversion invariant_neg as [cpu_less invariant_neg2].
+         apply imply_to_and in invariant_neg2.
+         inversion invariant_neg2 as [in_cpu no_jobs_hp].
+         assert (H : ~ (forall cpu : nat,
+                    cpu < num_cpus ->
+                    In cpu (seq 0 num_cpus) ->
+                    exists jhigh : job,
+                      hp jhigh j sched' 0 /\
+                      nth cpu (cpumap' sched' 0) None = Some jhigh)).
+         unfold not. intros.
+         specialize (H cpu cpu_less in_cpu).
+         apply no_jobs_hp. apply H.
+
 
 (* Definitions for APA affinity restoration *)
 
 (* Per-task affinities *)
 Definition task_affinity (alpha: affinity) :=
    forall (tsk: sporadic_task) (j1 j2: job),
-       job_of j1 tsk /\ job_of j2 tsk -> alpha j1 = alpha j2.
+       job_of j1 = Some tsk /\ job_of j2 = Some tsk -> alpha j1 = alpha j2.
 
 Definition inter : set nat -> set nat -> set nat := set_inter eq_nat_dec.
 
@@ -87,20 +151,20 @@ Definition restrict (tsk_i: sporadic_task) (ts: taskset)
     /\ task_affinity alpha'
     /\ (forall (tsk: sporadic_task) (j: job) (j_i: job),
          In tsk ts /\ In tsk_i ts
-         /\ job_of j tsk /\ job_of j_i tsk_i
+         /\ job_of j = Some tsk /\ job_of j_i = Some tsk_i
          -> alpha' j = inter (alpha j) (alpha j_i)).
 
 (* Service invariant from APA paper *)
 Lemma APA_service_invariant :
-    forall (num_cpus: nat) (sched: schedule) (hp: higher_priority)
+    forall (num_cpus: nat) (sched: schedule) (hp: higher_priority) (cpumap: processor_list)
            (ts: taskset) (alpha: affinity) (alpha': affinity) (tsk_i: sporadic_task)
            (j: job) (t: time),
-               apa_ident_mp num_cpus sched alpha hp
+               apa_ident_mp num_cpus sched hp cpumap alpha
                /\ In tsk_i ts
                /\ task_affinity alpha /\ task_affinity alpha'
                /\ restrict tsk_i ts alpha alpha'
-               -> exists (sched': schedule),
-                      (apa_ident_mp num_cpus sched' alpha' hp
+               -> exists (sched': schedule) (cpumap': processor_list),
+                      (apa_ident_mp num_cpus sched' hp cpumap' alpha'
                        /\ service sched j t >= service sched' j t).
 Proof.
     intros.
