job.v
@@ -1,40 +1,28 @@
-Require Import Coq.Lists.List.
+Add LoadPath "/home/felipec/dev/coq/rt-scheduling-spec".
+Require Import task.
 
-(* A task represents a single execution unit *)
-Record job : Type :=
-  { job_id: nat; (* allows multiple jobs with same parameters *)
+Section Job.
+
+Record job_data : Type :=
+  {
+    job_id: nat; (* job_id allows multiple jobs with same parameters *)
     job_cost: nat;
-    job_deadline: nat
+    job_deadline: nat; (* relative deadline *)
+    job_of: option sporadic_task (* Whether a job is spawned by a particular task *)
   }.
 
-(* Restrictions on job parameters *)
-Record valid_job (j: job) : Prop :=
-  { job_cost_positive: job_cost j > 0;
-    job_cost_le_deadline: job_cost j <= job_deadline j;
-    job_deadline_positive: job_deadline j > 0
+(* A job represents a single execution unit. *)
+Record job : Type :=
+  { jd:> job_data;
+
+    (* Properties of a job *)
+    job_cost_positive: job_cost jd > 0;
+    job_cost_le_deadline: job_cost jd <= job_deadline jd;
+    job_deadline_positive: job_deadline jd > 0;
+    job_task_parameters : forall (tsk: sporadic_task),
+                              job_of jd = Some tsk ->
+                                  (job_cost jd <= task_cost tsk
+                                  /\ job_deadline jd = task_deadline tsk)
   }.
 
-(* Sporadic Task Model *)
-Record sporadic_task : Type :=
-  { task_id: nat; (* allows multiple tasks with same parameters *)
-    task_cost: nat;
-    task_period : nat;
-    task_deadline: nat
-  }.
-
-Definition taskset := list sporadic_task.
-
-(* Jobs spawned by a task *)
-Axiom job_of : job -> sporadic_task -> Prop.
-Axiom task_parameters :
-    forall (j: job) (tsk: sporadic_task),
-        job_of j tsk ->
-            (job_cost j <= task_cost tsk
-            /\ job_deadline j = task_deadline tsk).
-
-(* Models for task deadlines *)
-Definition implicit_deadline_model (ts: taskset) : Prop :=
-    forall (tsk: sporadic_task), In tsk ts -> task_deadline tsk = task_period tsk.
-Definition restricted_deadline_model (ts: taskset) : Prop :=
-    forall (tsk: sporadic_task), In tsk ts -> task_deadline tsk <= task_period tsk.
-Definition arbitrary_deadline_model (ts: taskset) : Prop := True.
+End Job.
