schedule.v
@@ -1,67 +1,96 @@
 Add LoadPath "/home/felipec/dev/coq/rt-scheduling-spec".
 Require Import job.
+Require Import task.
 Require Import Coq.Lists.List.
+Require Import Coq.Arith.Gt.
 Require Import helper.
 
 (* Integer time *)
 Definition time := nat.
 
 (* Set of all possible job arrival sequences *)
-Definition arrival_seq := job -> time -> Prop.
+Definition arrival_sequence := job -> time -> Prop.
 
 (* Whether a particular arrival sequence is induced by a task set *)
-Definition ts_arrival_seq (ts: taskset) (arr: arrival_seq) : Prop :=
+Definition ts_arrival_sequence (ts: taskset) (arr: arrival_sequence) : Prop :=
     forall (j: job) (t: time),
-        arr j t -> (exists tsk: sporadic_task, job_of j tsk /\ List.In tsk ts).
+        arr j t -> (exists tsk: sporadic_task, job_of j = Some tsk /\ List.In tsk ts).
 
 (* Sporadic arrival times *)
-Definition periodic_task_model (ts: taskset) (arr: arrival_seq) : Prop :=
+Definition periodic_task_model (ts: taskset) (arr: arrival_sequence) : Prop :=
     forall (j1: job) (j2: job) (tsk: sporadic_task) (t: time) (t': time),
             (arr j1 t /\ arr j2 t' /\ t < t'
-            /\ job_of j1 tsk /\ job_of j2 tsk)
+            /\ job_of j1 = Some tsk /\ job_of j2 = Some tsk)
             -> t' = t + task_period tsk.
 
 (* Periodic arrival times *)
-Definition sporadic_task_model (ts: taskset) (arr: arrival_seq) : Prop :=
+Definition sporadic_task_model (ts: taskset) (arr: arrival_sequence) : Prop :=
     forall (j1: job) (j2: job) (tsk: sporadic_task) (t: time) (t': time),
             (arr j1 t /\ arr j2 t' /\ t < t'
-            /\ job_of j1 tsk /\ job_of j2 tsk)
+            /\ job_of j1 = Some tsk /\ job_of j2 = Some tsk)
             -> t' >= t + task_period tsk.
 
 (* Whether a job arrives at time t *)
-Definition arrived (arr: arrival_seq) (j: job)  (t: time) : Prop :=
+Definition arrived (arr: arrival_sequence) (j: job)  (t: time) : Prop :=
     exists (t_0: time), t_0 <= t /\ arr j t_0.
 
-Definition schedule := job -> time -> nat.
-
-(* Returns the arrival sequence of a particular schedule *)
-Axiom arr_seq_of : schedule -> arrival_seq.
+Record schedule_data : Type :=
+  {
+    (* service provided to a job at time t *)
+    service_at: job -> time -> nat; 
+    (* arrival sequence of the schedule *)
+    arr_seq: arrival_sequence
+  }.
 
 (* Service received by a job in a schedule, up to time t (inclusive) *)
-Fixpoint service (sched: schedule) (j: job) (t: time) : nat:=
+Fixpoint service (sched: schedule_data) (j: job) (t: time) : nat:=
   match t with
-      | 0 => sched j 0
-      | S t => service sched j t + sched j (S t)
+      | 0 => service_at sched j 0
+      | S t => service sched j t + service_at sched j (S t)
   end.
 
+(* Whether a job is scheduled at time t *)
+Definition scheduled (sched: schedule_data) (j: job) (t: time) : Prop :=
+    service_at sched j t > 0.
+
 (* Whether a job has completed at time t *)
-Definition completed (sched: schedule) (j: job) (t: time) : Prop :=
-    service sched j t = job_cost j.
+Definition completed (sched: schedule_data) (j: job) (t: time) : Prop :=
+    t > 0 /\ service sched j (t-1) = job_cost j.
 
 (* Whether a job is pending and not scheduled at time t *)
-Definition backlogged (sched: schedule) (j: job) (t: time) : Prop :=
-    sched j t = 0 /\ ~ completed sched j t.
+Definition backlogged (sched: schedule_data) (j: job) (t: time) : Prop :=
+    ~scheduled sched j t /\ ~completed sched j t.
 
-(* A job can only be scheduled if it arrived *)
-Axiom task_must_arrive_to_exec :
-    forall (j: job) (sched: schedule) (t: time),
-        sched j t > 0 -> arrived (arr_seq_of sched) j t.
+Record schedule : Type :=
+  {
+    sd:> schedule_data;
 
-(* A job cannot execute anymore after it completed *)
-Axiom completed_task_does_not_exec :
-    forall (sched: schedule) (j: job) (t_comp: time),
-        completed sched j t_comp ->
-            forall (t: time), t >= t_comp -> sched j t = 0.
+    (* Additional properties that a schedule must satisfy *)
+
+    (* 1) A job can only be scheduled if it arrived *)
+    task_must_arrive_to_exec :
+        forall (j: job) (t: time),
+            scheduled sd j t -> arrived (arr_seq sd) j t;
+
+    (* 2) A job cannot execute anymore after it completed *)
+    completed_task_does_not_exec :
+        forall (j: job) (t_comp: time),
+            completed sd j t_comp ->
+                forall (t: time), t >= t_comp -> ~ scheduled sd j t
+  }.
+
+Lemma backlogged_no_service : forall (sched: schedule_data) (j: job) (t: time),
+    backlogged sched j t -> service_at sched j t = 0.
+Proof.
+    intros sched j t j_backlogged.
+    unfold backlogged in j_backlogged.
+    inversion j_backlogged as [not_scheduled _].
+    unfold scheduled in not_scheduled.
+    assert (H := gt_0_eq (service_at sched j t)).
+    inversion H as [case1 | case2].
+        contradiction.
+        rewrite case2. reflexivity.
+Qed.
 
 (* Absolute time of completion for a job in a particular schedule *)
 Definition job_response_time (sched: schedule) (j: job) (t: time) :=
@@ -70,7 +99,7 @@ Definition job_response_time (sched: schedule) (j: job) (t: time) :=
 (* Worst-case response time of any job of a task, in any schedule *)
 Definition task_response_time (tsk: sporadic_task) (t: time) :=
     forall (j: job) (sched: schedule) (t: time),
-        job_of j tsk /\ greatest_nat t (job_response_time sched j).
+        job_of j = Some tsk /\ greatest_nat t (job_response_time sched j).
 
 (* Arrival time that generates the worst-case response time *)
 Definition critical_instant (tsk: sporadic_task) (sched: schedule) (t: time) :=
@@ -78,4 +107,10 @@ Definition critical_instant (tsk: sporadic_task) (sched: schedule) (t: time) :=
 
 (* Whether a schedule only contains jobs of a task set *)
 Definition schedule_of_taskset (sched: schedule) (ts: taskset) : Prop :=
-    forall (j: job) (t: time), sched j t > 0 -> (exists tsk, In tsk ts /\ job_of j tsk).
+    forall (j: job) (t: time), scheduled sched j t -> (exists tsk, In tsk ts /\ job_of j = Some tsk).
+
+Lemma no_completed_tasks_at_time_zero : forall (sched: schedule) (j: job) , ~completed sched j 0.
+Proof.
+    unfold not. intros.
+    inversion H. inversion H0.
+Qed.
