liulayland.v
@@ -2,6 +2,7 @@ Add LoadPath "/home/felipec/dev/coq/rt-scheduling-spec".
 Require Import Coq.Lists.List.
 Require Import Coq.Arith.Lt.
 Require Import job.
+Require Import task.
 Require Import schedule.
 Require Import identmp.
 Require Import priority.
@@ -11,18 +12,20 @@ Section LiuLayland.
 Variable ts: taskset.
 Variable sched: schedule.
 Variable hp: higher_priority.
-Axiom RM_priority : fixed_priority hp RM. (* Rate-monotonic priority *)
-Axiom uniprocessor : ident_mp 1 sched hp. (* Uniprocessor system *)
-Axiom jobs_from_taskset: schedule_of_taskset sched ts. (* All jobs come from task set *)
-Axiom arr_seq_from_ts: ts_arrival_seq ts (arr_seq_of sched). (* Arrival sequence from task set *)
-Axiom periodic_tasks: periodic_task_model ts (arr_seq_of sched).
-Axiom implicit_deadlines: implicit_deadline_model ts.
+Variable cpumap: processor_list.
+
+Hypothesis RM_priority : fixed_priority hp RM. (* Rate-monotonic priority *)
+Hypothesis uniprocessor : ident_mp 1 sched hp cpumap. (* Uniprocessor system *)
+Hypothesis jobs_from_taskset: schedule_of_taskset sched ts. (* All jobs come from task set *)
+Hypothesis arr_seq_from_ts: ts_arrival_sequence ts (arr_seq sched). (* Arrival sequence from task set *)
+Hypothesis periodic_tasks: periodic_task_model ts (arr_seq sched).
+Hypothesis implicit_deadlines: implicit_deadline_model ts.
 
 (* Simpler scheduling invariant for uniprocessor (eliminates cpu mapping) *)
 Lemma uni_simpler_invariant :
       forall (jlow : job) (t : time),
           backlogged sched jlow t
-              <-> exists jhigh : job, hp jhigh jlow sched t /\ sched jhigh t = 1.
+              <-> exists jhigh : job, hp jhigh jlow sched t /\ scheduled sched jhigh t.
 Proof.
   intros.
   assert (H1 := uniprocessor).
