task.v
@@ -1,0 +1,25 @@
+Add LoadPath "/home/felipec/dev/coq/rt-scheduling-spec".
+Require Import List.
+
+Section Task.
+
+(* Sporadic Task Model *)
+Record sporadic_task : Type :=
+  { task_id: nat; (* allows multiple tasks with same parameters *)
+    task_cost: nat;
+    task_period : nat;
+    task_deadline: nat (* relative deadline *)
+  }.
+
+Definition taskset := list sporadic_task.
+
+(* Models for task deadlines *)
+Definition implicit_deadline_model (ts: taskset) : Prop :=
+    forall (tsk: sporadic_task), In tsk ts -> task_deadline tsk = task_period tsk.
+
+Definition restricted_deadline_model (ts: taskset) : Prop :=
+    forall (tsk: sporadic_task), In tsk ts -> task_deadline tsk <= task_period tsk.
+
+Definition arbitrary_deadline_model (ts: taskset) : Prop := True.
+
+End Task.
